Model/Expr.dfy
@@ -1,0 +1,209 @@
+module Model_Expr {
+
+  import opened Utils
+  import opened MapFunction
+
+  datatype Expr = 
+    | MXor(e1: Expr, e2: Expr)
+    | MAnd(e1: Expr, e2: Expr)
+    | MOr(e1: Expr, e2: Expr)
+    | MInv(e: Expr)
+    | MIden(e: Expr)
+    | MConst(value: bool)
+    | MInput(ref: nat)
+    | MState(ref: nat)
+  {
+    predicate RefValid(il: nat, sl: nat)
+    {
+      match this
+      case MXor(e1, e2) => e1.RefValid(il, sl) && e2.RefValid(il, sl)
+      case MAnd(e1, e2) => e1.RefValid(il, sl) && e2.RefValid(il, sl)
+      case MOr(e1, e2) => e1.RefValid(il, sl) && e2.RefValid(il, sl)
+      case MInv(e) => e.RefValid(il, sl)
+      case MIden(e) => e.RefValid(il, sl)
+      case MConst(v) => true
+      case MInput(ref) => ref < il
+      case MState(ref) => ref < sl
+    }
+
+    predicate SIValid(si: SI)
+    {
+      RefValid(|si.inputs|, |si.state|)
+    }
+
+    function Evaluate(si: SI): (result: bool)
+      requires SIValid(si)
+    {
+      match this
+      case MXor(e1, e2) => Xor(e1.Evaluate(si), e2.Evaluate(si))
+      case MAnd(e1, e2) => e1.Evaluate(si) && e2.Evaluate(si)
+      case MOr(e1, e2) => e1.Evaluate(si) || e2.Evaluate(si)
+      case MInv(e) => !e.Evaluate(si)
+      case MIden(e) => e.Evaluate(si)
+      case MConst(v) => v
+      case MInput(r) => si.inputs[r]
+      case MState(r) => si.state[r]
+    }
+
+  }
+
+  datatype G<T> =
+    | GSingle(v: T)
+    | GSeq(s: seq<G>)
+
+  datatype Unary = Zero
+
+  function ToBase<T>(ge: G<T>): G<Unary>
+  {
+    match ge
+    case GSingle(v) => G<Unary>.GSingle(Zero)
+    case GSeq(s) => G<Unary>.GSeq(seq(|s|, (i: nat) requires i < |s| => ToBase(s[i])))
+  }
+
+  opaque predicate GExprSIValid(ge: G<Expr>, si: SI)
+  {
+    match ge
+    case GSingle(e) => e.SIValid(si)
+    case GSeq(s) => forall i: nat :: i < |s| ==> GExprSIValid(s[i], si)
+  }
+
+  opaque function GExprEvaluate(ge: G<Expr>, si: SI): (gb: G<bool>)
+    requires GExprSIValid(ge, si)
+    ensures ToBase(gb) == ToBase(ge)
+  {
+    reveal GExprSIValid();
+    var gb := match ge
+      case GSingle(e) => G<bool>.GSingle(e.Evaluate(si))
+      case GSeq(s) => G<bool>.GSeq(seq(|s|, (i: nat) requires i < |s| => GExprEvaluate(s[i], si)));
+    assert ToBase(gb) == ToBase(ge);
+    gb
+  }
+
+  predicate ToBaseComponentsEqual<T, U>(ge1: G<T>, ge2: G<U>)
+    requires ToBase(ge1) == ToBase(ge2)
+  {
+    match ge1
+    case GSingle(v) => (
+      assert ge2.GSingle?;
+      true
+    )
+    case GSeq(s) => (
+      assert |ToBase(ge1).s| == |ge1.s|;
+      forall i: nat :: i < |s| ==> ToBase(ge1.s[i]) == ToBase(ge2.s[i])
+    )
+  }
+
+  lemma ToBaseEqualSeqLength<T, U>(ge1: G<T>, ge2: G<U>)
+    requires ToBase(ge1) == ToBase(ge2)
+    requires ge1.GSeq?
+    ensures |ge1.s| == |ge2.s|
+  {
+    assert |ToBase(ge1).s| == |ToBase(ge2).s|;
+  }
+
+  lemma ToBaseEqualSeq<T, U>(ge1: G<T>, ge2: G<U>, index: nat)
+    requires ge1.GSeq?
+    requires index < |ge1.s|
+    requires ToBase(ge1) == ToBase(ge2)
+    ensures ge2.GSeq?
+    ensures |ge1.s| == |ge2.s|
+    ensures ToBase(ge1.s[index]) == ToBase(ge2.s[index])
+  {
+    assert |ToBase(ge1).s| == |ge1.s|;
+    assert |ToBase(ge2).s| == |ge2.s|;
+    assert ToBase(ge1.s[index]) == ToBase(ge1).s[index];
+  }
+
+  lemma ToBaseEqual<T, U>(ge1: G<T>, ge2: G<U>)
+    requires ToBase(ge1) == ToBase(ge2)
+    ensures ToBaseComponentsEqual(ge1, ge2)
+  {
+    match ge1
+    case GSingle(v) => {
+      assert ge2.GSingle?;
+      //true
+    }
+    case GSeq(s) => {
+      assert |ToBase(ge1).s| == |ge1.s|;
+      assert |ToBase(ge2).s| == |ge2.s|;
+      forall i: nat | i < |s|
+        ensures ToBase(ge1.s[i]) == ToBase(ge2.s[i])
+      {
+        assert ToBase(ge1).s[i] == ToBase(ge1.s[i]);
+      }
+    }
+  }
+
+  //datatype ExprType =
+  //  | ETBase(e: Expr)
+  //  | ETSeq(ets: seq<ExprType>)
+  //{
+  //  predicate SIValid(si: SI)
+  //  {
+  //    match this
+  //    case ETBase(e) => e.SIValid(si)
+  //    case ETSeq(ets) => forall i: nat :: i < |ets| ==> ets[i].SIValid(si)
+  //  }
+  //  function Evaluate(si: SI): ValType
+  //  {
+  //    match this
+  //    case ETBase(e) => VTBase(e.Evaluate(si))
+  //    case ETSeq(ets) => VTSeq(seq(|ets|, (i: nat) requires i < |ets| => ets[i].Evaluate(si)))
+  //  }
+  //}
+
+  //opaque predicate ExprsSIValid(es: seq<Expr>, si: SI)
+  //{
+  //  forall i: nat :: i < |es| ==> es[i].SIValid(si)
+  //}
+
+  //opaque function ExprsEvaluate(es: seq<Expr>, si: SI): (r: seq<bool>)
+  //  requires ExprsSIValid(es, si)
+  //  ensures |r| == |es|
+  //{
+  //  reveal ExprsSIValid();
+  //  seq(|es|, (i: nat) requires i < |es| => es[i].Evaluate(si))
+  //}
+
+
+  //datatype Soe = Soe(
+  //  input_width: nat,
+  //  outputs: seq<Expr>,
+  //  state: seq<Expr>
+  //)
+  //{
+
+  //  opaque predicate Valid()
+  //  {
+  //    && (forall o_index: nat :: o_index < |outputs| ==> outputs[o_index].RefValid(input_width, |state|))
+  //    && (forall s_index: nat :: s_index < |state| ==> state[s_index].RefValid(input_width, |state|))
+  //  }
+
+  //  opaque function Evaluate(si: SI): (so: SO)
+  //    requires Valid()
+  //    requires |si.inputs| == input_width
+  //    requires |si.state| == |state|
+  //    ensures |so.outputs| == |outputs|
+  //    ensures |so.state| == |state|
+  //  {
+  //    reveal Valid();
+  //    var outputs := seq(|outputs|, (o_index: nat) requires o_index < |outputs| => outputs[o_index].Evaluate(si));
+  //    var new_state := seq(|state|, (s_index: nat) requires s_index < |state| => state[s_index].Evaluate(si));
+  //    SO(outputs, new_state)
+  //  }
+
+  //}
+
+  //ghost opaque predicate SoeUFEquiv(soe: Soe, uf: UpdateFunction)
+  //  requires soe.Valid()
+  //  requires uf.Valid()
+  //{
+  //  && (soe.input_width == uf.input_width)
+  //  && (|soe.outputs| == uf.output_width)
+  //  && (|soe.state| == uf.state_width)
+  //  && (forall si: SI :: |si.inputs| == uf.input_width && |si.state| == uf.state_width ==>
+  //    && uf.sf.requires(si)
+  //    && (soe.Evaluate(si) == uf.sf(si)))
+  //}
+
+}
