Model/Mux2.dfy
@@ -1,0 +1,138 @@
+module Model_Mux2 {
+
+  import opened Model_Expr
+  import opened MapFunction
+  
+  function BaseMux2Expr(sel: Expr, a: Expr, b: Expr): (e: Expr)
+  {
+    var notsel := MInv(sel);
+    var mux2 := MOr(MAnd(notsel, a), MAnd(sel, b));
+    mux2
+  }
+
+  function BaseMux2(sel: bool, a: bool, b: bool): bool
+  {
+    if sel then b else a
+  }
+
+  lemma BaseMux2Equiv(sel: Expr, a: Expr, b: Expr, si: SI)
+    requires sel.SIValid(si)
+    requires a.SIValid(si)
+    requires b.SIValid(si)
+    ensures
+      var mux := BaseMux2Expr(sel, a, b);
+      var sel_val := sel.Evaluate(si);
+      var a_val := a.Evaluate(si);
+      var b_val := b.Evaluate(si);
+      && mux.SIValid(si)
+      && (mux.Evaluate(si) == BaseMux2(sel_val, a_val, b_val))
+  {
+    var sel_val := sel.Evaluate(si);
+    var a_val := a.Evaluate(si);
+    var b_val := b.Evaluate(si);
+    var notsel := MInv(sel);
+    var mux2 := MOr(MAnd(notsel, a), MAnd(sel, b));
+    assert sel.Evaluate(si) == sel_val;
+    assert a.Evaluate(si) == a_val;
+    assert b.Evaluate(si) == b_val;
+    assert notsel.Evaluate(si) == !sel_val;
+    assert mux2.Evaluate(si) == (!sel_val && a_val) || (sel_val && b_val);
+  }
+
+  opaque function Mux2Expr(sel: Expr, a: G<Expr>, b: G<Expr>): (r: G<Expr>)
+    requires ToBase(a) == ToBase(b)
+    ensures ToBase(a) == ToBase(r)
+  {
+    match a
+    case GSingle(e) => GSingle(BaseMux2Expr(sel, a.v, b.v))
+    case GSeq(s) => GSeq(seq(|s|, (i: nat) requires i < |s| =>
+      ToBaseEqual(a, b);
+      assert |ToBase(a).s| == |ToBase(b).s|;
+      Mux2Expr(sel, a.s[i], b.s[i])))
+  }
+
+  function Mux2(sel: bool, a: G<bool>, b: G<bool>): (r: G<bool>)
+    requires ToBase(a) == ToBase(b)
+    ensures ToBase(a) == ToBase(r)
+  {
+    if sel then b else a
+  }
+
+  lemma Mux2Equiv(sel: Expr, a: G<Expr>, b: G<Expr>, si: SI)
+    requires sel.SIValid(si)
+    requires ToBase(a) == ToBase(b)
+    requires GExprSIValid(a, si)
+    requires GExprSIValid(b, si)
+    ensures
+      var mux := Mux2Expr(sel, a, b);
+      var sel_val := sel.Evaluate(si);
+      var a_val := GExprEvaluate(a, si);
+      var b_val := GExprEvaluate(b, si);
+      && ToBase(a) == ToBase(a_val)
+      && ToBase(a) == ToBase(b_val)
+      && GExprSIValid(mux, si)
+      && (GExprEvaluate(mux, si) == Mux2(sel_val, a_val, b_val))
+  {
+    var mux := Mux2Expr(sel, a, b);
+    var sel_val := sel.Evaluate(si);
+    var a_val := GExprEvaluate(a, si);
+    var b_val := GExprEvaluate(b, si);
+    var t := ToBase(a);
+    assert ToBase(a_val) == t;
+    assert ToBase(mux) == t;
+    assert ToBase(b_val) == t;
+    match a
+    case GSingle(v) => {
+      assert a.v.SIValid(si) && b.v.SIValid(si) by {
+        reveal GExprSIValid();
+      }
+      BaseMux2Equiv(sel, a.v, b.v, si);
+      assert GExprSIValid(mux, si) by {
+        reveal Mux2Expr();
+        assert mux.v.SIValid(si);
+        reveal GExprSIValid();
+      }
+      assert (GExprEvaluate(mux, si) == Mux2(sel_val, a_val, b_val)) by {
+        reveal Mux2Expr();
+        reveal GExprEvaluate();
+      }
+    }
+    case GSeq(s) => {
+      ToBaseEqualSeqLength(a_val, b_val);
+      ToBaseEqualSeqLength(a, mux);
+      assert |a_val.s| == |b_val.s|;
+      forall i: nat | i < |s|
+        ensures |mux.s| == |a.s|
+        ensures GExprSIValid(mux.s[i], si)
+        ensures |a_val.s| == |a.s|
+        ensures |b_val.s| == |a.s|
+        ensures ToBase(a_val.s[i]) == ToBase(b_val.s[i])
+        ensures GExprEvaluate(mux.s[i], si) == Mux2(sel_val, a_val.s[i], b_val.s[i])
+      {
+        ToBaseEqualSeq(a, b, i);
+        ToBaseEqualSeq(a, a_val, i);
+        ToBaseEqualSeq(a, b_val, i);
+        assert GExprSIValid(a.s[i], si) && GExprSIValid(b.s[i], si) by {
+          reveal GExprSIValid();
+        }
+        Mux2Equiv(sel, a.s[i], b.s[i], si);
+        assert mux.s[i] == Mux2Expr(sel, a.s[i], b.s[i]) by {
+          reveal Mux2Expr();
+        }
+        assert GExprSIValid(mux.s[i], si);
+        assert && a_val.s[i] == GExprEvaluate(a.s[i], si)
+               && b_val.s[i] == GExprEvaluate(b.s[i], si) by {
+          reveal GExprEvaluate();
+        }
+        assert (GExprEvaluate(mux.s[i], si) == Mux2(sel_val, a_val.s[i], b_val.s[i]));
+      }
+      assert GExprSIValid(mux, si) by {
+        reveal GExprSIValid();
+      }
+      assert (GExprEvaluate(mux, si) == Mux2(sel_val, a_val, b_val)) by {
+        reveal GExprEvaluate();
+      }
+    }
+  }
+
+}
